compiler/binary/pure_frontendProgScript.sml
@@ -133,6 +133,7 @@ val r = translate spec_one_def;
 val r = translate specialise_each_def;
 val r = translate specialise_def;
 val r = translate cheap_def;
+val r = translate App_Lam_to_Lets_def;
 
 val r = translate_no_ind inline_def;
 
